AwsCryptographicMaterialProviders/dafny/AwsCryptographyKeyStoreAdmin/src/AwsCryptographyKeyStoreAdminOperations.dfy
@@ -482,10 +482,6 @@ module AwsCryptographyKeyStoreAdminOperations refines AbstractAwsCryptographyKey
     assume {:axiom} keyManagerStrat.Modifies < MutationLie();
     assume {:axiom} keyManagerStrat.Modifies !! systemKey.Modifies;
 
-    :- Need(
-      keyManagerStrat.SupportHV1(),
-      Types.KeyStoreAdminException(message := "At this time, Mutations do not support KeyManagementStrategy#AwsKmsSimple.")
-    );
     var internalInput := KSAApplyMutation.InternalApplyMutationInput(
       MutationToken := input.MutationToken,
       PageSize := input.PageSize,
